iso: Add dummy Memory modules

examples/dynamic_isolation/etc/rvcore.cuttlesim.cpp
@@ -8,6 +8,11 @@
 
 #define DMEM_SIZE (static_cast<std::size_t>(1) << 25)
 
+struct dram {
+  std::unique_ptr<bits<32>[]> mem;
+  std::optional<struct_mem_req> last;
+}
+
 struct bram {
   std::unique_ptr<bits<32>[]> mem;
   std::optional<struct_mem_req> last;
@@ -35,28 +40,6 @@ struct bram {
         ((dEn[2'0_d] ? data : current) & 0x32'000000ff_x) |
         ((dEn[2'1_d] ? data : current) & 0x32'0000ff00_x) |
         ((dEn[2'2_d] ? data : current) & 0x32'00ff0000_x) |
-        ((dEn[2'3_d] ? data : current) & 0x32'ff000000_x);
-    }
-
-    last.reset();
-    return std::optional<struct_mem_resp>{{
-        .byte_en = dEn, .addr = addr, .data = current
-      }};
-  }
-
-  bool put(std::optional<struct_mem_req> req) {
-    if (!req.has_value() || last.has_value())
-      return false;
-
-    last = *req;
-    return true;
-  }
-
-  struct_mem_output getput(struct_mem_input req) {
-    std::optional<struct_mem_resp> get_response = get(bool(req.get_ready));
-    bool put_ready = put(req.put_valid ? std::optional<struct_mem_req>{req.put_request} : std::nullopt);
-    return struct_mem_output{
-      .get_valid = bits<1>{get_response.has_value()},
       .put_ready = bits<1>{put_ready},
       .get_response = get_response.value_or(struct_mem_resp{})
     };
