examples/dynamic_isolation/Memory.v
@@ -7,10 +7,16 @@ Require Import DynamicIsolation.Scoreboard.
 Require Import DynamicIsolation.Multiplier.
 
 Require Import DynamicIsolation.External.
+Require Import DynamicIsolation.Lift.
 Require Import DynamicIsolation.Tactics.
 Require Import DynamicIsolation.Interfaces.
 
 (* Heavily inspired by http://csg.csail.mit.edu/6.175/labs/project-part1.html *)
+
+Definition post_t := unit.
+Definition var_t := string.
+Definition fn_name_t := string.
+
 
 Module CacheTypes.
   Import Common.
@@ -31,7 +37,10 @@ Module CacheTypes.
        struct_fields := [("core_id" , bits_t 1);
                          ("cache_type", enum_t cache_type);
                          ("addr"    , addr_t);
-                         ("MSI_state"   , enum_t MSI)] |}.
+                         ("MSI_state"   , enum_t MSI);
+                         ("tmp_req", struct_t mem_req)
+                        ] 
+    |}.
 
   Definition cache_mem_resp :=
     {| struct_name := "cache_mem_resp";
@@ -45,12 +54,12 @@ Module CacheTypes.
   Module FifoCacheMemReq <: Fifo.
     Definition T:= struct_t cache_mem_req.
   End FifoCacheMemReq.
-  Module CacheMemReq := Fifo1 FifoMemReq.
+  Module CacheMemReq := Fifo1 FifoCacheMemReq.
 
   Module FifoCacheMemResp <: Fifo.
     Definition T:= struct_t cache_mem_resp.
   End FifoCacheMemResp.
-  Module CacheMemResp := Fifo1 FifoMemResp.
+  Module CacheMemResp := Fifo1 FifoCacheMemResp.
 
   Definition cache_mem_msg_tag :=
     {| enum_name := "cache_mem_msg_tag";
@@ -64,6 +73,29 @@ Module CacheTypes.
                          ("req" , struct_t cache_mem_req);
                          ("resp" , struct_t cache_mem_resp)
                         ] |}.
+
+  (* TODO: We simplify:  *)
+
+
+  Definition log_num_sets := 12.
+  Definition log_tag_size := 18. (* 32 - 2 - 12 *)
+
+  Definition cache_tag_t := bits_t log_tag_size. (* TODO  *)
+  Definition cache_index_t := bits_t log_num_sets.
+  (* TODO: avoiding Koika arrays for now. This should be an array based on the block size *)
+  Definition cache_line_t := bits_t 32. 
+
+
+  (* TODO: figure out syntax to write as a function of log size *)
+  Definition getTag {reg_t}: UInternalFunction reg_t empty_ext_fn_t :=
+    {{ fun getTag (addr: bits_t 32) : cache_tag_t =>
+         addr[|5`d14|:+18]
+    }}.
+
+  Definition getIndex {reg_t}: UInternalFunction reg_t empty_ext_fn_t :=
+    {{ fun getIndex (addr: bits_t 32) : cache_tag_t =>
+         addr[|5`d2|:+12]
+    }}.
 
 End CacheTypes.
 
@@ -91,12 +123,12 @@ Module MessageFifo1.
 
   Definition enq_resp : UInternalFunction reg_t empty_ext_fn_t :=
     {{ fun enq_resp (resp: struct_t cache_mem_resp) : bits_t 0 =>
-         respQueue.(CacheMemResp.enq)()
+         respQueue.(CacheMemResp.enq)(resp)
     }}.
 
   Definition enq_req : UInternalFunction reg_t empty_ext_fn_t :=
-    {{ fun enq_req (resp: struct_t cache_mem_req) : bits_t 0 =>
-         reqQueue.(CacheMemReq.enq)()
+    {{ fun enq_req (req: struct_t cache_mem_req) : bits_t 0 =>
+         reqQueue.(CacheMemReq.enq)(req)
     }}.
 
   Definition has_resp : UInternalFunction reg_t empty_ext_fn_t :=
@@ -144,7 +176,7 @@ Module MessageFifo1.
        else
            let req_opt := reqQueue.(CacheMemReq.peek)() in
            struct cache_mem_msg {| type := enum cache_mem_msg_tag {| Req |};
-                                   resp := get(req_opt, data)
+                                   req := get(req_opt, data)
                                 |}
    }}.
 
@@ -205,6 +237,10 @@ Module MessageRouter.
 
   Import CacheTypes.
 
+  Definition Sigma := empty_Sigma.
+  Definition ext_fn_t := empty_ext_fn_t.
+  Definition rule := rule R Sigma.
+
   (* ===================== Message routing rules ============================== *)
   Definition memToCore : uaction reg_t empty_ext_fn_t :=
     {{ let msg := FromProto.(MessageFifo1.deq)() in
@@ -223,7 +259,7 @@ Module MessageRouter.
        else (* Resp *)
          let resp := get(msg, resp) in
          if (get(resp, core_id) == Ob~0) then
-           if (get(req, cache_type) == enum cache_type {| imem |}) then
+           if (get(resp, cache_type) == enum cache_type {| imem |}) then
              ToCore0I.(MessageFifo1.enq_resp)(resp)
            else
              ToCore0D.(MessageFifo1.enq_resp)(resp)
@@ -298,200 +334,183 @@ Module MessageRouter.
     {{ fun searchResponses (tiebreaker : bits_t 2) : maybe (struct_t cache_mem_msg) =>
          let foundMsg := Ob~0 in
          let msg := {invalid (struct_t cache_mem_msg)}() in
-         when (!foundMsg) do (
-           let curResp := getResp (tiebreaker) in
+         (when (!foundMsg) do (
+           let curResp := getResp (tiebreaker) in 
             when (get(curResp, valid)) do (
               set foundMsg := Ob~1;
-              set msg := get(curResp, data);
-              write0(internal routerTieBreaker, tieBreaker + |2`d1|)
+              set msg := {valid (struct_t cache_mem_msg)} (get(curResp, data));
+              write0(internal routerTieBreaker, tiebreaker + |2`d1|)
             )
-          );
-         when (!foundMsg) do (
-           let curResp := getResp (tieBreaker+|2`d1|) in
-           when (get(curResp, valid)) do (
-             set foundMsg := Ob~1;
-             set msg := get(curResp, data);
-             write0(internal routerTieBreaker, tieBreaker + |2`d2|)
-           )
-         );
-         when (!foundMsg) do (
-           let curResp := getResp (tieBreaker+|2`d2|) in
-           when (get(curResp, valid)) do (
-             set foundMsg := Ob~1;
-             set msg := get(curResp, data);
-             write0(internal routerTieBreaker, tieBreaker + |2`d3|)
-           )
-         );
-         when (!foundMsg) do (
-           let curResp := getResp (tieBreaker+|2`d3|) in
-           when (get(curResp, valid)) do (
-             set foundMsg := Ob~1;
-             set msg := get(curResp, data);
-             write0(internal routerTieBreaker, tieBreaker + |2`d4|)
-           )
-         )
+         ));
+         (when (!foundMsg) do (
+            let curResp := getResp (tiebreaker+|2`d1|) in
+            when (get(curResp, valid)) do (
+              set foundMsg := Ob~1;
+              set msg := {valid (struct_t cache_mem_msg)} (get(curResp, data));
+              write0(internal routerTieBreaker, tiebreaker + |2`d2|)
+            )
+          ));
+         (when (!foundMsg) do (
+            let curResp := getResp (tiebreaker+|2`d2|) in
+            when (get(curResp, valid)) do (
+              set foundMsg := Ob~1;
+              set msg := {valid (struct_t cache_mem_msg)} (get(curResp, data));
+              write0(internal routerTieBreaker, tiebreaker + |2`d3|)
+            )
+          ));
+         (when (!foundMsg) do (
+            let curResp := getResp (tiebreaker+|2`d3|) in
+            when (get(curResp, valid)) do (
+              set foundMsg := Ob~1;
+              set msg := {valid (struct_t cache_mem_msg)} (get(curResp, data));
+              write0(internal routerTieBreaker, tiebreaker + |2`d4|)
+            )
+          ));
+         msg
      }}.
 
-  (* ======= Search for responses, starting with tieBreaker ====== *)
+  (* ======= Search for responses, starting with tiebreaker ====== *)
   Definition searchRequests : UInternalFunction reg_t empty_ext_fn_t :=
-    {{ fun searchRequests (tieBreaker : bits_t 2) : maybe (struct_t cache_mem_msg) =>
+    {{ fun searchRequests (tiebreaker : bits_t 2) : maybe (struct_t cache_mem_msg) =>
          let foundMsg := Ob~0 in
          let msg := {invalid (struct_t cache_mem_msg)}() in
-         when (!foundMsg) do (
-           let curReq := getReq (tieBreaker) in
+         (when (!foundMsg) do (
+           let curReq := getReq (tiebreaker) in
             when (get(curReq, valid)) do (
               set foundMsg := Ob~1;
-              set msg := get(curReq, data);
-              write0(internal routerTieBreaker, tieBreaker + |2`d1|)
+              set msg := curReq;
+              write0(internal routerTieBreaker, tiebreaker + |2`d1|)
             )
-          );
-         when (!foundMsg) do (
-           let curReq := getReq (tieBreaker+|2`d1|) in
+          ));
+         (when (!foundMsg) do (
+           let curReq := getReq (tiebreaker+|2`d1|) in
            when (get(curReq, valid)) do (
              set foundMsg := Ob~1;
-             set msg := get(curReq, data);
-             write0(internal routerTieBreaker, tieBreaker + |2`d2|)
+             set msg := curReq;
+             write0(internal routerTieBreaker, tiebreaker + |2`d2|)
            )
-         );
-         when (!foundMsg) do (
-           let curReq := getReq (tieBreaker+|2`d2|) in
+         ));
+         (when (!foundMsg) do (
+           let curReq := getReq (tiebreaker+|2`d2|) in
            when (get(curReq, valid)) do (
              set foundMsg := Ob~1;
-             set msg := get(curReq, data);
-             write0(internal routerTieBreaker, tieBreaker + |2`d3|)
+             set msg := curReq;
+             write0(internal routerTieBreaker, tiebreaker + |2`d3|)
            )
-         );
-         when (!foundMsg) do (
-           let curReq := getReq (tieBreaker+|2`d3|) in
+         ));
+         (when (!foundMsg) do (
+           let curReq := getReq (tiebreaker+|2`d3|) in
            when (get(curReq, valid)) do (
              set foundMsg := Ob~1;
-             set msg := get(curReq, data);
-             write0(internal routerTieBreaker, tieBreaker + |2`d4|)
+             set msg := curReq;
+             write0(internal routerTieBreaker, tiebreaker + |2`d4|)
            )
-         )
+         ));
+         msg
      }}.
 
   Definition coreToMem : uaction reg_t empty_ext_fn_t :=
-    {{ let tieBreaker := read0(internal routerTieBreaker) in
+    {{ let tiebreaker := read0(internal routerTieBreaker) in
        (* Search for requests, starting with tieBreaker *)
-       let msg := searchResponses (tieBreaker) in
-       if (get(msg, valid)) then
+       let msg_opt := searchResponses (tiebreaker) in
+       if (get(msg_opt, valid)) then
          (* enqueue *)
+         let msg := get(msg_opt,data) in
          ToProto.(MessageFifo1.enq_resp)(get(msg,resp))
        else
-       (* Search for responses, starting with tieBreaker *)
-         let msg := searchRequests (tieBreaker) in
-         if (get(msg,valid)) then
+       (* Search for responses, starting with tiebreaker *)
+         let msg_opt := searchRequests (tiebreaker) in
+         if (get(msg_opt,valid)) then
+           let msg := get(msg_opt, data) in
            ToProto.(MessageFifo1.enq_req)(get(msg,req))
          else
-           write0(internal routerTieBreaker, tieBreaker + |2`d1|)
+           write0(internal routerTieBreaker, tiebreaker + |2`d1|)
     }}.
+
+  Inductive rule_name_t :=
+  | Rl_MemToCore
+  | Rl_CoreToMem
+  .
+
+  Definition tc_memToCore := tc_rule R Sigma memToCore <: rule.
+  Definition tc_coreToMem := tc_rule R Sigma coreToMem <: rule.
+
+  Definition rules (rl: rule_name_t) : rule :=
+    match rl with
+    | Rl_MemToCore => tc_memToCore
+    | Rl_CoreToMem => tc_coreToMem
+    end.
+
+  Definition schedule : Syntax.scheduler pos_t rule_name_t :=
+    Rl_MemToCore |> Rl_CoreToMem |> done.
 
 End MessageRouter.
 
-Module WIPMemory <: Memory_sig External.
+Module Type CacheParams.
+  Parameter core_id : Common.core_id_t.
+  Parameter cache_type : enum_t CacheTypes.cache_type.
+End CacheParams.
+
+Module Cache (Params: CacheParams).
+  Import CacheTypes.
   Import Common.
 
-  (* This memory has two L1 I&D caches, a message router, and protocol processor, and the main memory.
-   * TODO: next we will add a L2 cache.
-   *)
+  (* Hard-coded for now: direct-mapped cache: #sets = #blocks; word-addressable *)
+  
+  Definition cache_row := 
+    {| struct_name := "cache_row";
+       struct_fields := [("tag", cache_tag_t);
+                         ("data", cache_line_t);
+                         ("flag", enum_t MSI)] |}.
 
-  (* TODO: In theory we would do this in a more modular way, but we simplify for now.
-   *)
-  Inductive internal_reg_t' : Type :=
-  | core0IToRouter (state: MessageFifo1.reg_t)
-  | core0DToRouter (state: MessageFifo1.reg_t)
-  | core1IToRouter (state: MessageFifo1.reg_t)
-  | core1DToRouter (state: MessageFifo1.reg_t)
-  | RouterToCore0I (state: MessageFifo1.reg_t)
-  | RouterToCore0D (state: MessageFifo1.reg_t)
-  | RouterToCore1I (state: MessageFifo1.reg_t)
-  | RouterToCore1D (state: MessageFifo1.reg_t)
-  | RouterToProto (state: MessageFifo1.reg_t)
-  | ProtoToRouter (state: MessageFifo1.reg_t)
-  | Router_internal (state: MessageRouter.internal_reg_t)
+  Definition mshr_tag :=
+    {| enum_name := "mshr_tag";
+       enum_members := vect_of_list ["Ready"; "SendFillReq"; "WaitFillResp"];
+       enum_bitpatterns := vect_of_list [Ob~0~0; Ob~0~1; Ob~1~0] 
+    |}.
+
+  (* TODO *)
+  Definition MSHR_t :=
+    {| struct_name := "MSHR"; 
+       struct_fields := [("mshr_tag", enum_t mshr_tag);
+                         ("req", struct_t mem_req)
+                        ] |}.
+  
+  Inductive internal_reg_t :=
+  | requestsQ (state: MemReq.reg_t)
+  | responsesQ (state: MemResp.reg_t)
+  | MSHR
   .
 
-  Definition internal_reg_t := internal_reg_t'.
+  Instance FiniteType_internal_reg_t : FiniteType internal_reg_t := _.
 
   Definition R_internal (idx: internal_reg_t) : type :=
     match idx with
-    | core0IToRouter st => MessageFifo1.R st
-    | core0DToRouter st => MessageFifo1.R st
-    | core1IToRouter st => MessageFifo1.R st
-    | core1DToRouter st => MessageFifo1.R st
-    | RouterToCore0I st => MessageFifo1.R st
-    | RouterToCore0D st => MessageFifo1.R st
-    | RouterToCore1I st => MessageFifo1.R st
-    | RouterToCore1D st => MessageFifo1.R st
-    | RouterToProto st => MessageFifo1.R st
-    | ProtoToRouter st => MessageFifo1.R st
-    | Router_internal st => MessageRouter.R_internal st
+    | requestsQ st => MemReq.R st
+    | responsesQ st => MemResp.R st
+    | mshr => struct_t MSHR_t
     end.
 
   Definition r_internal (idx: internal_reg_t) : R_internal idx :=
     match idx with
-    | core0IToRouter st => MessageFifo1.r st
-    | core0DToRouter st => MessageFifo1.r st
-    | core1IToRouter st => MessageFifo1.r st
-    | core1DToRouter st => MessageFifo1.r st
-    | RouterToCore0I st => MessageFifo1.r st
-    | RouterToCore0D st => MessageFifo1.r st
-    | RouterToCore1I st => MessageFifo1.r st
-    | RouterToCore1D st => MessageFifo1.r st
-    | RouterToProto st => MessageFifo1.r st
-    | ProtoToRouter st => MessageFifo1.r st
-    | Router_internal st => MessageRouter.r_internal st
+    | requestsQ st => MemReq.r st
+    | responsesQ st => MemResp.r st
+    | mshr => value_of_bits (Bits.zero)
     end.
 
-  Instance FiniteType_internal_reg_t : FiniteType internal_reg_t := _.
 
   Inductive reg_t :=
-  | toIMem0 (state: MemReq.reg_t)
-  | toIMem1 (state: MemReq.reg_t)
-  | toDMem0 (state: MemReq.reg_t)
-  | toDMem1 (state: MemReq.reg_t)
-  | fromIMem0 (state: MemResp.reg_t)
-  | fromIMem1 (state: MemResp.reg_t)
-  | fromDMem0 (state: MemResp.reg_t)
-  | fromDMem1 (state: MemResp.reg_t)
-  | internal (r: internal_reg_t)
+  | fromMem (state: MessageFifo1.reg_t)
+  | toMem (state: MessageFifo1.reg_t)
+  | internal (state: internal_reg_t)
   .
-
-  Definition R (idx: reg_t) :=
+  
+  Definition R (idx: reg_t) : type :=
     match idx with
-    | toIMem0 st => MemReq.R st
-    | toIMem1 st => MemReq.R st
-    | toDMem0 st => MemReq.R st
-    | toDMem1 st => MemReq.R st
-    | fromIMem0 st => MemResp.R st
-    | fromIMem1 st => MemResp.R st
-    | fromDMem0 st => MemResp.R st
-    | fromDMem1 st => MemResp.R st
+    | fromMem st => MessageFifo1.R st
+    | toMem st => MessageFifo1.R st
     | internal st => R_internal st
     end.
-
-  Definition r idx : R idx :=
-    match idx with
-    | toIMem0 st => MemReq.r st
-    | toIMem1 st => MemReq.r st
-    | toDMem0 st => MemReq.r st
-    | toDMem1 st => MemReq.r st
-    | fromIMem0 st => MemResp.r st
-    | fromIMem1 st => MemResp.r st
-    | fromDMem0 st => MemResp.r st
-    | fromDMem1 st => MemResp.r st
-    | internal st => r_internal st
-    end.
-
-  Definition ext_fn_t := External.ext_fn_t.
-  Definition Sigma := External.Sigma.
-  Definition rule := rule R Sigma.
-  (* Definition sigma := External.sigma. *)
-
-  Definition MMIO_UART_ADDRESS := Ob~0~1~0~0~0~0~0~0~0~0~0~0~0~0~0~0~0~0~0~0~0~0~0~0~0~0~0~0~0~0~0~0.
-  Definition MMIO_LED_ADDRESS  := Ob~0~1~0~0~0~0~0~0~0~0~0~0~0~0~0~0~0~0~0~0~0~0~0~0~0~0~0~0~0~1~0~0.
-
 
   Notation "'__internal__' instance " :=
     (fun reg => internal ((instance) reg)) (in custom koika at level 1, instance constr at level 99).
@@ -499,7 +518,246 @@ Module WIPMemory <: Memory_sig External.
     (USugar (UCallModule instance _ method args))
       (in custom koika at level 1, method constr, args custom koika_args at level 99).
 
+  Definition Sigma := empty_Sigma.
+  Definition ext_fn_t := empty_ext_fn_t.
+
+  (* Ready -> SendFillReq;
+     SendFillReq -> WaitFillResp;
+     WaitFillResp -> Ready
+  *)
+
+  (* Definition downgrade : uaction reg_t empty_ext_fn_t. Admitted. *)
+
+  Definition dummy_mem_req : struct_t mem_req := value_of_bits (Bits.zero).
+  Definition dummy_mem_resp : struct_t mem_resp := value_of_bits (Bits.zero).
+
+  (* TOOD: for now, just assume miss and skip cache and forward to memory *)
+  Definition dummy_process_request : uaction reg_t empty_ext_fn_t :=
+    {{ 
+        let mshr := read0(internal MSHR) in
+        guard(get(mshr,mshr_tag) == enum mshr_tag {| Ready |});
+        let req := (__internal__ requestsQ).(MemReq.deq)() in
+        write0(internal MSHR, struct MSHR_t {| mshr_tag := enum mshr_tag {| SendFillReq |};
+                                               req := req
+                                            |})
+                                               
+    }}.
+
+  Definition byte_en_to_msi_state : UInternalFunction reg_t empty_ext_fn_t := 
+    {{ fun byte_en_to_msi_state (byte_en: bits_t 4) : enum_t MSI => 
+         match byte_en with
+         | Ob~0~0~0~0 => enum MSI {| S |}
+         return default : enum MSI {| M |}
+         end
+    }}.
+
+  Definition core_id := Params.core_id.
+  Definition cache_type := Params.cache_type.
+  Definition fake : struct_t cache_mem_req. Admitted.
+
+  Definition dummy_SendFillReq : uaction reg_t empty_ext_fn_t :=
+    {{  
+        let mshr := read0(internal MSHR) in
+        guard(get(mshr,mshr_tag) == enum mshr_tag {| SendFillReq |});
+        let mshr_req := get(mshr,req) in
+        toMem.(MessageFifo1.enq_req)(
+                  struct cache_mem_req {| core_id := (#core_id);
+                                          cache_type := (`UConst (cache_type)`);
+                                          addr := get(mshr_req, addr);
+                                          MSI_state := (match get(mshr_req,byte_en) with
+                                                        | Ob~0~0~0~0 => enum MSI {| S |}
+                                                        return default : enum MSI {| M |}
+                                                        end);
+                                          tmp_req := mshr_req
+                                       |});
+        write0(internal MSHR, struct MSHR_t {| mshr_tag := enum mshr_tag {| WaitFillResp |};
+                                               req := mshr_req
+                                            |})
+    }}.
+ 
+  (* TODO: move to Std *)
+  Section Maybe.
+    Context (tau: type).
+
+    Definition fromMaybe {reg_t fn}: UInternalFunction reg_t fn := 
+      {{ fun fromMaybe (default: tau) (val: maybe tau) : tau =>
+           if get(val, valid) then get(val, data)
+           else default 
+      }}. 
+  End Maybe.
+             
+
+  (* If Store: do nothing in response *)
+  (* If Load: send response *)
+  Definition hit : UInternalFunction reg_t empty_ext_fn_t :=
+    {{ fun hit (req: struct_t mem_req) (row: struct_t cache_row) : enum_t mshr_tag =>
+         let new_state := enum mshr_tag {| Ready |} in
+         if (get(req, byte_en) == Ob~0~0~0~0) then
+           (__internal__ responsesQ).(MemResp.enq)(
+             struct mem_resp {| addr := get(req, addr);
+                                data := get(row,data);
+                                byte_en := get(req, byte_en)
+                             |})
+         else (* TODO: commit data *)
+           pass
+         ;
+         new_state
+    }}.
+
+  Definition dummy_WaitFillResp : uaction reg_t empty_ext_fn_t :=
+    {{  
+        let mshr := read0(internal MSHR) in
+        guard(get(mshr,mshr_tag) == enum mshr_tag {| WaitFillResp |} &&
+              fromMem.(MessageFifo1.has_resp)());
+        let resp := get(fromMem.(MessageFifo1.deq)(),resp) in
+
+        let req := get(mshr, req) in
+        let row := struct cache_row {| tag := getTag(get(req, addr));
+                                       data := {fromMaybe data_t}(|32`d0|, get(resp,data))
+                                    |} in
+        ignore(hit(req, row)); 
+        write0(internal MSHR, struct MSHR_t {| mshr_tag := enum mshr_tag {| Ready |};
+                                               req := (`UConst dummy_mem_req`)
+                                            |})
+    }}.
+        
+  Definition req: UInternalFunction reg_t empty_ext_fn_t :=
+    {{ fun req (r: struct_t mem_req) : bits_t 0 =>
+         let mshr := read0(internal MSHR) in
+         guard(get(mshr,mshr_tag) == enum mshr_tag {| Ready |});
+         (__internal__ requestsQ).(MemReq.enq)(r)
+    }}.
+
+  Definition resp: UInternalFunction reg_t empty_ext_fn_t :=
+    {{ fun resp () : struct_t mem_resp =>
+         (__internal__ responsesQ).(MemResp.deq)()
+    }}.
+
+  Inductive rule_name_t :=
+  | Rl_ProcessRequest
+  | Rl_SendFillReq
+  | Rl_WaitFillResp
+  .
+
+  Definition rule := rule R Sigma.
+
+  Definition tc_processRequest := tc_rule R Sigma (dummy_process_request) <: rule.
+  Definition tc_sendFillReq := tc_rule R Sigma (dummy_SendFillReq) <: rule.
+  Definition tc_waitFillResp := tc_rule R Sigma (dummy_WaitFillResp) <: rule.
+
+  Definition rules (rl: rule_name_t) : rule :=
+    match rl with
+    | Rl_ProcessRequest => tc_processRequest
+    | Rl_SendFillReq => tc_sendFillReq
+    | Rl_WaitFillResp => tc_waitFillResp
+    end.
+
+  Definition schedule : Syntax.scheduler pos_t rule_name_t :=
+    Rl_ProcessRequest |> Rl_SendFillReq |> Rl_WaitFillResp |> done.
+                   
+End Cache.
+
+Module ProtocolProcessor.
+  Import Common.
+  Import CacheTypes.
+
+  (* TODO: Should be a DDR3_Req or similar, and should parameterise based on DDR3AddrSize/DataSize *)
+  Inductive reg_t :=
+  | FromRouter (state: MessageFifo1.reg_t)
+  | ToRouter (state: MessageFifo1.reg_t)
+  | ToMem (state: MemReq.reg_t)
+  | FromMem (state: MemResp.reg_t)
+  . 
+
+  Definition R (idx: reg_t) : type := 
+    match idx with
+    | FromRouter st => MessageFifo1.R st
+    | ToRouter st => MessageFifo1.R st
+    | ToMem st => MemReq.R st
+    | FromMem st => MemResp.R st
+    end.
+
+  Definition Sigma := empty_Sigma.
+  Definition ext_fn_t := empty_ext_fn_t.
+
+  (* For now: we assume everything is always invalid because the caches don't actually exist.  *)
+
+  Definition forward_req : uaction reg_t empty_ext_fn_t :=
+    {{ 
+        guard (!FromRouter.(MessageFifo1.has_resp)() &&
+                FromRouter.(MessageFifo1.has_req)()
+              );
+        let req := get(FromRouter.(MessageFifo1.deq)(),req) in
+        (* Tmp: just forward *)
+        ToMem.(MemReq.enq)(get(req, tmp_req))
+    }}.
+
+  Definition forward_resp_from_mem : uaction reg_t empty_ext_fn_t :=
+    {{ let resp := FromMem.(MemResp.deq)() in
+       FromMem.(MemResp.enq)(resp)
+    }}.
+
+  Inductive rule_name_t :=
+  | Rl_ForwardReq
+  | Rl_ForwardResp
+  .
+
+  Definition rule := rule R Sigma.
+
+  Definition tc_forwardReq := tc_rule R Sigma (forward_req) <: rule.
+  Definition tc_forwardResp := tc_rule R Sigma (forward_resp_from_mem) <: rule.
+
+  Definition rules (rl: rule_name_t) : rule :=
+    match rl with
+    | Rl_ForwardReq => tc_forwardReq
+    | Rl_ForwardResp => tc_forwardResp
+    end.
+
+  Definition schedule : Syntax.scheduler pos_t rule_name_t :=
+    Rl_ForwardReq |> Rl_ForwardResp |> done.
+                   
+     (*
+  Definition forward_resp : uaction reg_t empty_ext_fn_t :=
+    {{ 
+        guard (FromRouter.(MessageFifo1.has_resp)());
+        let resp := FromRouter.(MessageFifo1.deq)() in
+        let cid := get(resp, core_id) in
+        let idx := getIndex (get(resp, addr)) in
+        let resp_data := get(resp,data) in
+        if (get(resp_data, valid)) then
+          let req := struct mem_req {| addr := get(resp, addr);
+                                       data := get(resp_data, data);
+                                       byte_en := get(resp, byte_en)
+                                    |} in
+          ToMem.(MemReq.enq)(req)
+        else pass
+    }}.
+    *)
+
+
+End ProtocolProcessor.
+
+Module MainMem.
+  Import Common.
+  Inductive reg_t :=
+  | FromProto (state: MemReq.reg_t)
+  | ToProto   (state: MemResp.reg_t)
+  .
+
+  Definition R idx : type :=
+    match idx with
+    | FromProto st => MemReq.R st
+    | ToProto st => MemResp.R st
+    end.
+
   Import External.
+
+  Definition ext_fn_t := External.ext_fn_t.
+  Definition Sigma := External.Sigma.
+  Definition rule := rule R Sigma.
+
+  Definition MMIO_UART_ADDRESS := Ob~0~1~0~0~0~0~0~0~0~0~0~0~0~0~0~0~0~0~0~0~0~0~0~0~0~0~0~0~0~0~0~0.
+  Definition MMIO_LED_ADDRESS  := Ob~0~1~0~0~0~0~0~0~0~0~0~0~0~0~0~0~0~0~0~0~0~0~0~0~0~0~0~0~0~1~0~0.
 
   Definition memoryBus (m: memory) : UInternalFunction reg_t ext_fn_t :=
     {{ fun memoryBus (get_ready: bits_t 1) (put_valid: bits_t 1) (put_request: struct_t mem_req) : struct_t mem_output =>
@@ -508,7 +766,8 @@ Module WIPMemory <: Memory_sig External.
                         get_ready := get_ready;
                         put_valid := put_valid;
                         put_request := put_request |}) }}
-          | dmem => {{ let addr := get(put_request, addr) in
+          | _    => {{
+                      let addr := get(put_request, addr) in
                       let byte_en := get(put_request, byte_en) in
                       let is_write := byte_en == Ob~1~1~1~1 in
 
@@ -560,41 +819,338 @@ Module WIPMemory <: Memory_sig External.
                           put_valid := put_valid && is_mem;
                           put_request := put_request |})
                    }}
-          end` }}.
+          end` }} .
 
-  Definition mem (m: memory) : uaction reg_t ext_fn_t :=
-    let fromMem := match m with imem => fromIMem0 | dmem => fromDMem0 end in
-    let toMem := match m with imem => toIMem0 | dmem => toDMem0 end in
+  Definition mem : uaction reg_t ext_fn_t :=
+    let fromMem := ToProto in
+    let toMem := FromProto in
     {{
         let get_ready := fromMem.(MemResp.can_enq)() in
         let put_request_opt := toMem.(MemReq.peek)() in
         let put_request := get(put_request_opt, data) in
         let put_valid := get(put_request_opt, valid) in
-        let mem_out := {memoryBus m}(get_ready, put_valid, put_request) in
+        let mem_out := {memoryBus mainmem}(get_ready, put_valid, put_request) in
         (when (get_ready && get(mem_out, get_valid)) do fromMem.(MemResp.enq)(get(mem_out, get_response)));
         (when (put_valid && get(mem_out, put_ready)) do ignore(toMem.(MemReq.deq)()))
     }}.
 
-  Definition tc_imem := tc_rule R Sigma (mem imem) <: rule.
-  Definition tc_dmem := tc_rule R Sigma (mem dmem) <: rule.
+  Definition tc_mem := tc_rule R Sigma mem <: rule.
 
-  Inductive rule_name_t' :=
-  | Imem
-  | Dmem
+  Inductive rule_name_t :=
+  | Rl_mem
   .
-
-  Definition rule_name_t := rule_name_t'.
 
   Definition rules (rl: rule_name_t) : rule :=
     match rl with
-    | Imem           => tc_imem
-    | Dmem           => tc_dmem
+    | Rl_mem => tc_mem
     end.
 
-  Definition schedule : scheduler :=
-    Imem |> Dmem |> done.
+  Definition schedule : Syntax.scheduler pos_t rule_name_t :=
+    Rl_mem |> done.
 
-  Instance FiniteType_reg_t : FiniteType reg_t := _.
+End MainMem.
+
+Module WIPMemory <: Memory_sig External.
+  Import Common.
+
+  (* This memory has two L1 I&D caches, a message router, and protocol processor, and the main memory.
+   * TODO: next we will add a L2 cache.
+   *)
+
+  Import CacheTypes.
+
+  Module Params_Core0IMem <: CacheParams.
+    Definition core_id := Ob~0.
+    Definition cache_type : enum_t cache_type := Ob~0. (* imem *)
+  End Params_Core0IMem.
+
+  Module Params_Core0DMem <: CacheParams.
+    Definition core_id := Ob~0.
+    Definition cache_type : enum_t cache_type := Ob~1. (* dmem *)
+  End Params_Core0DMem.
+
+  Module Params_Core1IMem <: CacheParams.
+    Definition core_id := Ob~1.
+    Definition cache_type : enum_t cache_type := Ob~0. (* imem *)
+  End Params_Core1IMem.
+
+
+  Module Params_Core1DMem <: CacheParams.
+    Definition core_id := Ob~1.
+    Definition cache_type : enum_t cache_type := Ob~1. (* dmem *)
+  End Params_Core1DMem.
+
+  Module Core0IMem := Cache Params_Core0IMem.
+  Module Core0DMem := Cache Params_Core0DMem.
+  Module Core1IMem := Cache Params_Core1IMem.
+  Module Core1DMem := Cache Params_Core0DMem.
+
+
+  (* TODO: In theory we would do this in a more modular way, but we simplify for now.
+   *)
+  Inductive internal_reg_t' : Type :=
+  | core0IToRouter (state: MessageFifo1.reg_t)
+  | core0DToRouter (state: MessageFifo1.reg_t)
+  | core1IToRouter (state: MessageFifo1.reg_t)
+  | core1DToRouter (state: MessageFifo1.reg_t)
+  | RouterToCore0I (state: MessageFifo1.reg_t)
+  | RouterToCore0D (state: MessageFifo1.reg_t)
+  | RouterToCore1I (state: MessageFifo1.reg_t)
+  | RouterToCore1D (state: MessageFifo1.reg_t)
+  | RouterToProto (state: MessageFifo1.reg_t)
+  | ProtoToRouter (state: MessageFifo1.reg_t)
+  | ProtoToMem (state: MemReq.reg_t)
+  | MemToProto (state: MemResp.reg_t)
+  | Router_internal (state: MessageRouter.internal_reg_t)
+  | Core0I_internal (state: Core0IMem.internal_reg_t)
+  | Core0D_internal (state: Core0DMem.internal_reg_t)
+  | Core1I_internal (state: Core1IMem.internal_reg_t)
+  | Core1D_internal (state: Core1DMem.internal_reg_t)
+  .
+
+  Definition internal_reg_t := internal_reg_t'.
+
+  Definition R_internal (idx: internal_reg_t) : type :=
+    match idx with
+    | core0IToRouter st => MessageFifo1.R st
+    | core0DToRouter st => MessageFifo1.R st
+    | core1IToRouter st => MessageFifo1.R st
+    | core1DToRouter st => MessageFifo1.R st
+    | RouterToCore0I st => MessageFifo1.R st
+    | RouterToCore0D st => MessageFifo1.R st
+    | RouterToCore1I st => MessageFifo1.R st
+    | RouterToCore1D st => MessageFifo1.R st
+    | RouterToProto st => MessageFifo1.R st
+    | ProtoToRouter st => MessageFifo1.R st
+    | ProtoToMem st => MemReq.R st
+    | MemToProto st => MemResp.R st
+    | Router_internal st => MessageRouter.R_internal st
+    | Core0I_internal st => Core0IMem.R_internal st
+    | Core0D_internal st => Core0DMem.R_internal st
+    | Core1I_internal st => Core1IMem.R_internal st
+    | Core1D_internal st => Core1DMem.R_internal st
+    end.
+
+  Definition r_internal (idx: internal_reg_t) : R_internal idx :=
+    match idx with
+    | core0IToRouter st => MessageFifo1.r st
+    | core0DToRouter st => MessageFifo1.r st
+    | core1IToRouter st => MessageFifo1.r st
+    | core1DToRouter st => MessageFifo1.r st
+    | RouterToCore0I st => MessageFifo1.r st
+    | RouterToCore0D st => MessageFifo1.r st
+    | RouterToCore1I st => MessageFifo1.r st
+    | RouterToCore1D st => MessageFifo1.r st
+    | RouterToProto st => MessageFifo1.r st
+    | ProtoToRouter st => MessageFifo1.r st
+    | ProtoToMem st => MemReq.r st
+    | MemToProto st => MemResp.r st
+    | Router_internal st => MessageRouter.r_internal st
+    | Core0I_internal st => Core0IMem.r_internal st
+    | Core0D_internal st => Core0DMem.r_internal st
+    | Core1I_internal st => Core1IMem.r_internal st
+    | Core1D_internal st => Core1DMem.r_internal st
+    end.
+
+  Instance FiniteType_internal_reg_t : FiniteType internal_reg_t := _.
+
+  Inductive reg_t :=
+  | toIMem0 (state: MemReq.reg_t)
+  | toIMem1 (state: MemReq.reg_t)
+  | toDMem0 (state: MemReq.reg_t)
+  | toDMem1 (state: MemReq.reg_t)
+  | fromIMem0 (state: MemResp.reg_t)
+  | fromIMem1 (state: MemResp.reg_t)
+  | fromDMem0 (state: MemResp.reg_t)
+  | fromDMem1 (state: MemResp.reg_t)
+  | internal (r: internal_reg_t)
+  .
+
+  Definition R (idx: reg_t) :=
+    match idx with
+    | toIMem0 st => MemReq.R st
+    | toIMem1 st => MemReq.R st
+    | toDMem0 st => MemReq.R st
+    | toDMem1 st => MemReq.R st
+    | fromIMem0 st => MemResp.R st
+    | fromIMem1 st => MemResp.R st
+    | fromDMem0 st => MemResp.R st
+    | fromDMem1 st => MemResp.R st
+    | internal st => R_internal st
+    end.
+
+  Definition r idx : R idx :=
+    match idx with
+    | toIMem0 st => MemReq.r st
+    | toIMem1 st => MemReq.r st
+    | toDMem0 st => MemReq.r st
+    | toDMem1 st => MemReq.r st
+    | fromIMem0 st => MemResp.r st
+    | fromIMem1 st => MemResp.r st
+    | fromDMem0 st => MemResp.r st
+    | fromDMem1 st => MemResp.r st
+    | internal st => r_internal st
+    end.
+
+  Definition ext_fn_t := External.ext_fn_t.
+  Definition Sigma := External.Sigma.
+  Definition rule := rule R Sigma.
+  (* Definition sigma := External.sigma. *)
+
+  Notation "'__internal__' instance " :=
+    (fun reg => internal ((instance) reg)) (in custom koika at level 1, instance constr at level 99).
+  Notation "'(' instance ').(' method ')' args" :=
+    (USugar (UCallModule instance _ method args))
+      (in custom koika at level 1, method constr, args custom koika_args at level 99).
+
+  Import External.
+
+  (* =============== Lifts ================ *)
+
+  Section Core0_IMemLift.
+    Definition core0_imem_lift (reg: Core0IMem.reg_t) : reg_t :=
+      match reg with
+      | Core0IMem.fromMem st => (internal (RouterToCore0I st))
+      | Core0IMem.toMem st => (internal (core0IToRouter st))
+      | Core0IMem.internal st => (internal (Core0I_internal st))
+      end.
+
+    Definition Lift_core0_imem : RLift _ Core0IMem.reg_t reg_t Core0IMem.R R := ltac:(mk_rlift core0_imem_lift).
+    Definition FnLift_core0_imem : RLift _ Core0IMem.ext_fn_t ext_fn_t Core0IMem.Sigma Sigma := ltac:(lift_auto).
+
+  End Core0_IMemLift.
+
+  Section Core0_DMemLift.
+    Definition core0_dmem_lift (reg: Core0DMem.reg_t) : reg_t :=
+      match reg with
+      | Core0DMem.fromMem st => (internal (RouterToCore0D st))
+      | Core0DMem.toMem st => (internal (core0DToRouter st))
+      | Core0DMem.internal st => (internal (Core0D_internal st))
+      end.
+
+    Definition Lift_core0_dmem : RLift _ Core0DMem.reg_t reg_t Core0DMem.R R := ltac:(mk_rlift core0_dmem_lift).
+    Definition FnLift_core0_dmem : RLift _ Core0DMem.ext_fn_t ext_fn_t Core0DMem.Sigma Sigma := ltac:(lift_auto).
+
+  End Core0_DMemLift.
+
+  (* TODO: Core1 *)
+  Section MessageRouterLift.
+    Definition router_lift (reg: MessageRouter.reg_t) : reg_t := 
+    match reg with
+    | MessageRouter.FromCore0I st => (internal (core0IToRouter st))
+    | MessageRouter.FromCore0D st => (internal (core0DToRouter st))
+    | MessageRouter.FromCore1I st => (internal (core1IToRouter st))
+    | MessageRouter.FromCore1D st => (internal (core1DToRouter st))
+    | MessageRouter.ToCore0I st => (internal (RouterToCore0I st))
+    | MessageRouter.ToCore0D st => (internal (RouterToCore0D st))
+    | MessageRouter.ToCore1I st => (internal (RouterToCore1I st))
+    | MessageRouter.ToCore1D st => (internal (RouterToCore1D st))
+    | MessageRouter.ToProto st => (internal (RouterToProto st))
+    | MessageRouter.FromProto st => (internal (ProtoToRouter st))
+    | MessageRouter.internal st => (internal (Router_internal st))
+    end.
+
+    Definition Lift_router : RLift _ MessageRouter.reg_t reg_t MessageRouter.R R := ltac:(mk_rlift router_lift).
+    Definition FnLift_router : RLift _ MessageRouter.ext_fn_t ext_fn_t MessageRouter.Sigma Sigma := ltac:(lift_auto).
+    
+  End MessageRouterLift.
+
+  Section ProtocolProcessorLift.
+
+    Definition proto_lift (reg: ProtocolProcessor.reg_t) : reg_t :=
+    match reg with 
+    | ProtocolProcessor.FromRouter st => (internal (RouterToProto st))
+    | ProtocolProcessor.ToRouter st => (internal (ProtoToRouter st ))
+    | ProtocolProcessor.ToMem st => (internal (ProtoToMem st))
+    | ProtocolProcessor.FromMem st => (internal (MemToProto st))
+    end.
+
+    Definition Lift_proto : RLift _ ProtocolProcessor.reg_t reg_t ProtocolProcessor.R R := ltac:(mk_rlift proto_lift).
+    Definition FnLift_proto : RLift _ ProtocolProcessor.ext_fn_t ext_fn_t ProtocolProcessor.Sigma Sigma := ltac:(lift_auto).
+
+  End ProtocolProcessorLift.
+
+  Section MainMemLift.
+    Definition main_mem_lift (reg: MainMem.reg_t) : reg_t := 
+      match reg with
+      | MainMem.FromProto st => internal (ProtoToMem st)
+      | MainMem.ToProto st => internal (MemToProto st)
+      end.
+
+    Definition Lift_main_mem: RLift _ MainMem.reg_t reg_t MainMem.R R := ltac:(mk_rlift main_mem_lift).
+    Definition FnLift_main_mem: RLift _ MainMem.ext_fn_t ext_fn_t MainMem.Sigma Sigma := ltac:(lift_auto).
+  End MainMemLift.
+
+  (* TODO: slow *)
+  (* Instance FiniteType_reg_t : FiniteType reg_t := _. *)
+  Declare Instance FiniteType_reg_t : FiniteType reg_t.  
+  Instance EqDec_reg_t : EqDec reg_t := _.
+
+  Section Rules.
+    Inductive rule_name_t' :=
+    | Rl_Core0IMem (r: Core0IMem.rule_name_t)
+    | Rl_Core0DMem (r: Core0DMem.rule_name_t)
+    | Rl_Proto (r: ProtocolProcessor.rule_name_t)
+    | Rl_Router (r: MessageRouter.rule_name_t)
+    | Rl_MainMem (r: MainMem.rule_name_t)
+    .
+
+    Definition rule_name_t := rule_name_t'.
+
+    Definition core0I_rule_name_lift (rl: Core0IMem.rule_name_t) : rule_name_t :=
+      Rl_Core0IMem rl.
+
+    Definition core0D_rule_name_lift (rl: Core0DMem.rule_name_t) : rule_name_t :=
+      Rl_Core0DMem rl.
+
+    Definition proto_rule_name_lift (rl: ProtocolProcessor.rule_name_t) : rule_name_t :=
+      Rl_Proto rl.
+
+    Definition router_rule_name_lift (rl: MessageRouter.rule_name_t) : rule_name_t :=
+      Rl_Router rl.
+
+    Definition main_mem_name_lift (rl: MainMem.rule_name_t) : rule_name_t :=
+      Rl_MainMem rl.
+    
+    Definition core0I_rules (rl: Core0IMem.rule_name_t) : rule :=
+      lift_rule Lift_core0_imem FnLift_core0_imem (Core0IMem.rules rl).
+    Definition core0D_rules (rl: Core0DMem.rule_name_t) : rule :=
+      lift_rule Lift_core0_dmem FnLift_core0_dmem (Core0DMem.rules rl).
+    Definition proto_rules (rl: ProtocolProcessor.rule_name_t) : rule :=
+      lift_rule Lift_proto FnLift_proto (ProtocolProcessor.rules rl).
+    Definition router_rules (rl: MessageRouter.rule_name_t) : rule :=
+      lift_rule Lift_router FnLift_router (MessageRouter.rules rl).
+    Definition main_mem_rules (rl: MainMem.rule_name_t) : rule :=
+      lift_rule Lift_main_mem FnLift_main_mem (MainMem.rules rl).
+
+    Definition rules (rl: rule_name_t) : rule :=
+      match rl with
+      | Rl_Core0IMem r => core0I_rules r
+      | Rl_Core0DMem r => core0D_rules r
+      | Rl_Proto r => proto_rules r
+      | Rl_Router r => router_rules r
+      | Rl_MainMem r => main_mem_rules r
+     end.
+
+  End Rules.
+
+  Section Schedule.
+    Definition core0I_schedule := lift_scheduler core0I_rule_name_lift Core0IMem.schedule.
+    Definition core0D_schedule := lift_scheduler core0D_rule_name_lift Core0DMem.schedule.
+    Definition proto_schedule := lift_scheduler proto_rule_name_lift ProtocolProcessor.schedule.
+    Definition router_schedule := lift_scheduler router_rule_name_lift MessageRouter.schedule.
+    Definition main_mem_schedule := lift_scheduler main_mem_name_lift MainMem.schedule.
+
+    (* TODO: move this *)
+    Notation "r '||>' s" :=
+      (schedule_app r s)
+        (at level 99, s at level 99, right associativity).
+
+    Definition schedule :=
+      core0I_schedule ||> core0D_schedule ||> router_schedule ||> proto_schedule ||> main_mem_schedule.
+
+  End Schedule.
+
 End WIPMemory.
 
 
@@ -668,70 +1224,76 @@ Module SimpleMemory <: Memory_sig External.
 
   Import External.
 
-  Definition memoryBus (m: memory) : UInternalFunction reg_t ext_fn_t :=
+  Inductive simple_memory :=
+  | imem0
+  | dmem0
+  .
+
+  Definition memoryBus (m: simple_memory) : UInternalFunction reg_t ext_fn_t :=
     {{ fun memoryBus (get_ready: bits_t 1) (put_valid: bits_t 1) (put_request: struct_t mem_req) : struct_t mem_output =>
          `match m with
-          | imem => {{ extcall (ext_mem m) (struct mem_input {|
-                        get_ready := get_ready;
-                        put_valid := put_valid;
-                        put_request := put_request |}) }}
-          | dmem => {{ let addr := get(put_request, addr) in
-                      let byte_en := get(put_request, byte_en) in
-                      let is_write := byte_en == Ob~1~1~1~1 in
+          | imem0 => {{ extcall (ext_mem imem) (struct mem_input {|
+                         get_ready := get_ready;
+                         put_valid := put_valid;
+                         put_request := put_request |}) }}
+          | dmem0 => {{ let addr := get(put_request, addr) in
+                       let byte_en := get(put_request, byte_en) in
+                       let is_write := byte_en == Ob~1~1~1~1 in
 
-                      let is_uart := addr == #MMIO_UART_ADDRESS in
-                      let is_uart_read := is_uart && !is_write in
-                      let is_uart_write := is_uart && is_write in
+                       let is_uart := addr == #MMIO_UART_ADDRESS in
+                       let is_uart_read := is_uart && !is_write in
+                       let is_uart_write := is_uart && is_write in
 
-                      let is_led := addr == #MMIO_LED_ADDRESS in
-                      let is_led_write := is_led && is_write in
+                       let is_led := addr == #MMIO_LED_ADDRESS in
+                       let is_led_write := is_led && is_write in
 
-                      let is_mem := !is_uart && !is_led in
+                       let is_mem := !is_uart && !is_led in
 
-                      if is_uart_write then
-                        let char := get(put_request, data)[|5`d0| :+ 8] in
-                        let may_run := get_ready && put_valid && is_uart_write in
-                        let ready := extcall ext_uart_write (struct (Maybe (bits_t 8)) {|
-                          valid := may_run; data := char |}) in
-                        struct mem_output {| get_valid := may_run && ready;
-                                             put_ready := may_run && ready;
-                                             get_response := struct mem_resp {|
-                                               byte_en := byte_en; addr := addr;
-                                               data := |32`d0| |} |}
+                       if is_uart_write then
+                         let char := get(put_request, data)[|5`d0| :+ 8] in
+                         let may_run := get_ready && put_valid && is_uart_write in
+                         let ready := extcall ext_uart_write (struct (Maybe (bits_t 8)) {|
+                           valid := may_run; data := char |}) in
+                         struct mem_output {| get_valid := may_run && ready;
+                                              put_ready := may_run && ready;
+                                              get_response := struct mem_resp {|
+                                                byte_en := byte_en; addr := addr;
+                                                data := |32`d0| |} |}
 
-                      else if is_uart_read then
-                        let may_run := get_ready && put_valid && is_uart_read in
-                        let opt_char := extcall ext_uart_read (may_run) in
-                        let ready := get(opt_char, valid) in
-                        struct mem_output {| get_valid := may_run && ready;
-                                             put_ready := may_run && ready;
-                                             get_response := struct mem_resp {|
-                                               byte_en := byte_en; addr := addr;
-                                               data := zeroExtend(get(opt_char, data), 32) |} |}
+                       else if is_uart_read then
+                         let may_run := get_ready && put_valid && is_uart_read in
+                         let opt_char := extcall ext_uart_read (may_run) in
+                         let ready := get(opt_char, valid) in
+                         struct mem_output {| get_valid := may_run && ready;
+                                              put_ready := may_run && ready;
+                                              get_response := struct mem_resp {|
+                                                byte_en := byte_en; addr := addr;
+                                                data := zeroExtend(get(opt_char, data), 32) |} |}
 
-                      else if is_led then
-                        let on := get(put_request, data)[|5`d0|] in
-                        let may_run := get_ready && put_valid && is_led_write in
-                        let current := extcall ext_led (struct (Maybe (bits_t 1)) {|
-                          valid := may_run; data := on |}) in
-                        let ready := Ob~1 in
-                        struct mem_output {| get_valid := may_run && ready;
-                                             put_ready := may_run && ready;
-                                             get_response := struct mem_resp {|
-                                               byte_en := byte_en; addr := addr;
-                                               data := zeroExtend(current, 32) |} |}
+                       else if is_led then
+                         let on := get(put_request, data)[|5`d0|] in
+                         let may_run := get_ready && put_valid && is_led_write in
+                         let current := extcall ext_led (struct (Maybe (bits_t 1)) {|
+                           valid := may_run; data := on |}) in
+                         let ready := Ob~1 in
+                         struct mem_output {| get_valid := may_run && ready;
+                                              put_ready := may_run && ready;
+                                              get_response := struct mem_resp {|
+                                                byte_en := byte_en; addr := addr;
+                                                data := zeroExtend(current, 32) |} |}
 
-                      else
-                        extcall (ext_mem m) (struct mem_input {|
-                          get_ready := get_ready && is_mem;
-                          put_valid := put_valid && is_mem;
-                          put_request := put_request |})
+                       else
+                         extcall (ext_mem dmem) (struct mem_input {|
+                           get_ready := get_ready && is_mem;
+                           put_valid := put_valid && is_mem;
+                           put_request := put_request |})
                    }}
           end` }}.
 
-  Definition mem (m: memory) : uaction reg_t ext_fn_t :=
-    let fromMem := match m with imem => fromIMem0 | dmem => fromDMem0 end in
-    let toMem := match m with imem => toIMem0 | dmem => toDMem0 end in
+  (* TODO: not defined for main_mem *)
+  Definition mem (m: simple_memory) : uaction reg_t ext_fn_t :=
+    let fromMem := match m with imem0 => fromIMem0 | dmem0 => fromDMem0 end in
+    let toMem := match m with imem0 => toIMem0 | dmem0 => toDMem0 end in
     {{
         let get_ready := fromMem.(MemResp.can_enq)() in
         let put_request_opt := toMem.(MemReq.peek)() in
@@ -742,8 +1304,8 @@ Module SimpleMemory <: Memory_sig External.
         (when (put_valid && get(mem_out, put_ready)) do ignore(toMem.(MemReq.deq)()))
     }}.
 
-  Definition tc_imem := tc_rule R Sigma (mem imem) <: rule.
-  Definition tc_dmem := tc_rule R Sigma (mem dmem) <: rule.
+  Definition tc_imem := tc_rule R Sigma (mem imem0) <: rule.
+  Definition tc_dmem := tc_rule R Sigma (mem dmem0) <: rule.
 
   Inductive rule_name_t' :=
   | Imem
